sim stuff

src/computational_monads/simulation_semantics/constructions/logging/query_cache/basic.lean
@@ -31,23 +31,29 @@ section lookup
 def lookup (cache : query_cache spec) (i : spec.ι) (t : spec.domain i) :
   option (spec.range i) := cache i t
 
-variables (i : spec.ι) (t : spec.domain i)
+/-- Have `simp` normalize towards using `lookup` over direct application. -/
+@[simp] lemma apply_eq_lookup (i t) : cache i t = cache.lookup i t := rfl
 
-@[ext] protected lemma ext {spec : oracle_spec} {cache cache' : query_cache spec}
-  (h : ∀ (i : spec.ι) t, cache.lookup i t = cache'.lookup i t) : cache = cache' :=
+@[ext] protected lemma ext {cache cache' : query_cache spec}
+  (h : ∀ i t, cache.lookup i t = cache'.lookup i t) : cache = cache' :=
 funext (λ _, funext (λ _, h _ _))
 
-protected lemma ext_iff {spec : oracle_spec} {cache cache' : query_cache spec} :
-  cache = cache' ↔ ∀ (i : spec.ι) t, cache.lookup i t = cache'.lookup i t :=
+protected lemma ext_iff : cache = cache' ↔ ∀ i t, cache.lookup i t = cache'.lookup i t :=
 ⟨λ h i t, h ▸ rfl, query_cache.ext⟩
 
 lemma ne_iff_exists_lookup_ne : cache ≠ cache' ↔ ∃ i t, cache.lookup i t ≠ cache'.lookup i t :=
 function.ne_iff.trans ⟨λ h, let ⟨i, hi⟩ := h in let ⟨t, ht⟩ := function.ne_iff.1 hi in ⟨i, t, ht⟩,
   λ h, let ⟨i, t, ht⟩ := h in ⟨i, function.ne_iff.2 ⟨t, ht⟩⟩⟩
 
-lemma ne_of_lookup_ne (i : spec.ι) (t : spec.domain i)
-  (h : cache.lookup i t ≠ cache'.lookup i t) : cache ≠ cache' :=
+lemma ne_of_lookup_ne (i t) (h : cache.lookup i t ≠ cache'.lookup i t) : cache ≠ cache' :=
 (ne_iff_exists_lookup_ne cache cache').2 ⟨i, t, h⟩
+
+lemma lookup_ne_some_of_lookup_eq_none {i t} (h : cache.lookup i t = none)
+  (u : spec.range i) : cache.lookup i t ≠ some u :=
+λ hu, (option.some_ne_none u (hu.symm.trans h))
+
+lemma lookup_ne_none_of_lookup_eq_some {i t u} (h : cache.lookup i t = some u) :
+  cache.lookup i t ≠ none := λ hu, (option.some_ne_none u (h.symm.trans hu))
 
 end lookup
 
@@ -57,19 +63,30 @@ section is_fresh
 @[derive decidable]
 def is_fresh (i : spec.ι) (t : spec.domain i) := (cache.lookup i t).is_none = tt
 
-variables (i : spec.ι) (t : spec.domain i)
-
-@[simp] lemma lookup_eq_none_iff_is_fresh : cache.lookup i t = none ↔ cache.is_fresh i t :=
+@[simp] lemma lookup_eq_none_iff_is_fresh (i t) : cache.lookup i t = none ↔ cache.is_fresh i t :=
 by simp [is_fresh, option.is_none_iff_eq_none]
 
-@[simp] lemma none_eq_lookup_iff_is_fresh : none = cache.lookup i t ↔ cache.is_fresh i t :=
+@[simp] lemma none_eq_lookup_iff_is_fresh (i t) : none = cache.lookup i t ↔ cache.is_fresh i t :=
 eq_comm.trans (lookup_eq_none_iff_is_fresh cache i t)
 
 lemma is_fresh_of_lookup_eq_none {i t} (h : cache.lookup i t = none) : cache.is_fresh i t :=
 (lookup_eq_none_iff_is_fresh cache i t).1 h
 
+@[simp] lemma lookup_eq_none_of_is_fresh {i t} (h : cache.is_fresh i t) : cache.lookup i t = none :=
+(cache.lookup_eq_none_iff_is_fresh i t).2 h
+
 lemma not_is_fresh_of_lookup_eq_some {i t u} (h : cache.lookup i t = some u) :
   ¬ cache.is_fresh i t := by simp [is_fresh, h]
+
+lemma lookup_ne_some_of_is_fresh {i t} (h : cache.is_fresh i t) (u : spec.range i) :
+  cache.lookup i t ≠ some u := by simp [h]
+
+lemma is_fresh_of_is_fresh_of_lookup_eq {i t} (h : cache.is_fresh i t)
+  (h' : cache.lookup i t = cache'.lookup i t) : cache'.is_fresh i t :=
+begin
+  rw [← lookup_eq_none_iff_is_fresh] at ⊢ h,
+  exact h'.symm.trans h
+end
 
 end is_fresh
 
@@ -79,35 +96,68 @@ section is_cached
 @[derive decidable]
 def is_cached (i : spec.ι) (t : spec.domain i) := (cache.lookup i t).is_some = tt
 
-variables (i : spec.ι) (t : spec.domain i) (u : spec.range i)
+@[simp] lemma not_is_cached_iff_is_fresh (i t) : ¬ cache.is_cached i t ↔ cache.is_fresh i t :=
+by rw [is_cached, option.not_is_some_iff_eq_none, lookup_eq_none_iff_is_fresh]
 
-lemma is_cached_iff_exists_lookup_eq_some :
+@[simp]  lemma not_is_fresh_iff_is_cached (i t) : ¬ cache.is_fresh i t ↔ cache.is_cached i t :=
+by rw [← not_is_cached_iff_is_fresh, not_not]
+
+lemma not_is_cached_of_is_fresh {i t} (h : cache.is_fresh i t) : ¬ cache.is_cached i t :=
+(not_is_cached_iff_is_fresh cache i t).2 h
+
+lemma is_fresh_of_not_is_cached {i t} (h : ¬ cache.is_cached i t) : cache.is_fresh i t :=
+(not_is_cached_iff_is_fresh cache i t).1 h
+
+lemma not_is_fresh_of_is_cached {i t} (h : cache.is_cached i t) : ¬ cache.is_fresh i t :=
+(not_is_fresh_iff_is_cached cache i t).2 h
+
+lemma is_cached_of_not_is_fresh {i t} (h : ¬ cache.is_fresh i t) : cache.is_cached i t :=
+(not_is_fresh_iff_is_cached cache i t).1 h
+
+lemma is_cached_iff_exists_lookup_eq_some (i t) :
   cache.is_cached i t ↔ ∃ u, cache.lookup i t = some u :=
 by simp [is_cached, ← option.is_some_iff_exists]
+
+lemma not_is_fresh_iff_exists_lookup_eq_some (i t) :
+  ¬ cache.is_fresh i t ↔ ∃ u, cache.lookup i t = some u :=
+by simp [is_cached_iff_exists_lookup_eq_some]
 
 lemma is_cached_of_lookup_eq_some {i t u} (h : cache.lookup i t = some u) :
   cache.is_cached i t := (is_cached_iff_exists_lookup_eq_some cache i t).2 ⟨u, h⟩
 
+lemma lookup_eq_some_of_is_cached {i t} (h : cache.is_cached i t) :
+  ∃ u, cache.lookup i t = some u := (cache.is_cached_iff_exists_lookup_eq_some i t).1 h
+
 lemma not_is_cached_of_lookup_eq_none {i t} (h : cache.lookup i t = none) :
   ¬ cache.is_cached i t := by simp [is_cached, h]
 
-lemma is_cached_iff_not_is_fresh : cache.is_cached i t ↔ ¬ cache.is_fresh i t :=
-by {simp [is_cached, is_fresh], cases cache.lookup i t; simp}
+lemma lookup_eq_none_of_not_is_cached {i t} (h : ¬ cache.is_cached i t) :
+  cache.lookup i t = none := lookup_eq_none_of_is_fresh cache (is_fresh_of_not_is_cached _ h)
 
-@[simp] lemma lookup_ne_none_iff_is_cached : cache.lookup i t ≠ none ↔ cache.is_cached i t :=
-by simp [is_cached_iff_not_is_fresh]
+lemma lookup_ne_none_iff_is_cached (i t) :
+  cache.lookup i t ≠ none ↔ cache.is_cached i t := by simp
 
-@[simp] lemma lookup_ne_none_iff_exists_lookup_eq_some :
+lemma lookup_ne_none_iff_exists_lookup_eq_some {i t} :
   cache.lookup i t ≠ none ↔ ∃ u, cache.lookup i t = some u :=
-by rw [lookup_ne_none_iff_is_cached, is_cached_iff_exists_lookup_eq_some]
+by simp [is_cached_iff_exists_lookup_eq_some]
+
+@[simp] lemma some_get_or_else_lookup_of_is_cached {i t u} (h : cache.is_cached i t) :
+  some ((cache.lookup i t).get_or_else u) = cache.lookup i t :=
+let ⟨u, hu⟩ := lookup_eq_some_of_is_cached _ h in by simp [hu]
+
+lemma is_cached_of_is_cached_of_lookup_eq {i t} (h' : cache.is_cached i t)
+  (h : cache.lookup i t = cache'.lookup i t) : cache'.is_cached i t :=
+begin
+  rw [is_cached_iff_exists_lookup_eq_some] at h' ⊢,
+  exact let ⟨u, hu⟩ := h' in ⟨u, h.symm.trans hu⟩
+end
 
 end is_cached
 
 section init
 
 /-- `init spec` is the empty cache not containing any values yet (i.e. all are `none` still). -/
-@[inline, reducible] protected def init (spec : oracle_spec) :
-  query_cache spec := λ _ _, none
+protected def init (spec : oracle_spec) : query_cache spec := λ _ _, none
 
 variables (i : spec.ι) (t : spec.domain i)
 
@@ -117,7 +167,7 @@ instance : inhabited (query_cache spec) := ⟨∅⟩
 
 lemma init_apply' : (∅ : query_cache spec) i = λ _, none := rfl
 
-lemma init_apply : (∅ : query_cache spec) i t = none := rfl
+@[simp] lemma init_apply : (∅ : query_cache spec) i t = none := rfl
 
 @[simp] lemma lookup_init : lookup ∅ i t = none := rfl
 
@@ -127,113 +177,17 @@ lemma lookup_init_ne_some (u : spec.range i) : lookup ∅ i t ≠ some u := by s
 
 @[simp] lemma not_is_cached_init : ¬ is_cached ∅ i t := by simp [is_cached]
 
-@[simp] lemma eq_init_iff : cache = ∅ ↔ ∀ i t, cache.is_fresh i t :=
+@[simp] lemma eq_init_iff_forall_is_fresh : cache = ∅ ↔ ∀ i t, cache.is_fresh i t :=
 by simp [query_cache.ext_iff]
 
-lemma eq_init_iff' : cache = ∅ ↔ ∀ i t, cache.lookup i t = none :=
-by simp [query_cache.ext_iff]
+lemma eq_init_iff_forall_eq_none : cache = ∅ ↔ ∀ i t, cache.lookup i t = none := by simp
 
-lemma ne_init_iff : cache ≠ ∅ ↔ ∃ i t, cache.is_cached i t :=
-by simp [eq_init_iff, is_cached_iff_not_is_fresh]
+lemma ne_init_iff_exists_is_cached : cache ≠ ∅ ↔ ∃ i t, cache.is_cached i t := by simp
 
-lemma ne_init_iff' : cache ≠ ∅ ↔ ∃ i t u, cache.lookup i t = some u :=
-by simp [eq_init_iff, ne.def, ← is_cached_iff_not_is_fresh, is_cached_iff_exists_lookup_eq_some]
+lemma ne_init_iff_exists_eq_some : cache ≠ ∅ ↔ ∃ i t u, cache.lookup i t = some u :=
+by simp [is_cached_iff_exists_lookup_eq_some]
 
 end init
-
-section order -- TODO: `is_mono` typeclass for `sim_oracle`.
-
-/-- We say `cache ≤ cache'` for two query caches it every cached value in `cache` has the same
-value cached in `cache'`. For uncached values the corresponding value can be anything.
-We also have an `inf` operation that only returns values cached in both original caches. -/
-instance : semilattice_inf (query_cache spec) :=
-{ le := λ cache cache', ∀ i t u, cache.lookup i t = some u → cache'.lookup i t = some u,
-  le_refl := λ cache i t u h, h,
-  le_trans := λ cache cache' cache'' h h' i t u h'', h' i t u (h i t u h''),
-  le_antisymm := λ cache cache' h' h, query_cache.ext (λ i t,
-    begin
-      by_cases hi : cache.lookup i t = none,
-      { by_cases hi' : cache'.lookup i t = none,
-        { rw [hi, hi'] },
-        { obtain ⟨u, hu⟩ := option.ne_none_iff_exists'.1 hi',
-          refine (option.some_ne_none u ((h i t u hu).symm.trans hi)).elim } },
-      { exact let ⟨u, hu⟩ := option.ne_none_iff_exists'.1 hi in (hu.trans (h' i t u hu).symm) }
-    end),
-  inf := λ cache cache' i t, if cache.is_fresh i t ∨ cache'.is_fresh i t then none else
-    (if cache.lookup i t = cache'.lookup i t then cache.lookup i t else none),
-  inf_le_left := begin
-    refine λ cache cache' i t u hu, _,
-    by_cases h : cache.is_fresh i t ∨ cache'.is_fresh i t,
-    { exact (option.some_ne_none _ (hu.symm.trans (by simp [lookup, h]))).elim },
-    { have := (if_neg h).symm.trans hu,
-      simp [ite_eq_iff', imp_false] at this,
-      exact this.1 this.2 }
-  end,
-  inf_le_right := begin
-    refine λ cache cache' i t u hu, _,
-    by_cases h : cache.is_fresh i t ∨ cache'.is_fresh i t,
-    { exact (option.some_ne_none _ (hu.symm.trans (by simp [lookup, h]))).elim },
-    { have := (if_neg h).symm.trans hu,
-      simp [ite_eq_iff', imp_false] at this,
-      exact this.2.symm.trans (this.1 this.2) }
-  end,
-  le_inf := λ cache₁ cache₂ cache₃ h2 h3 i t u hu, trans (if_neg (not_or_distrib.2
-    ⟨cache₂.not_is_fresh_of_lookup_eq_some (h2 i t u hu), cache₃.not_is_fresh_of_lookup_eq_some
-      (h3 i t u hu)⟩)) (trans (if_pos ((h2 i t u hu).trans (h3 i t u hu).symm)) (h2 i t u hu)) }
-
-variables (i : spec.ι) (t : spec.domain i) (u : spec.range i)
-
-lemma le_iff : cache ≤ cache' ↔ ∀ i t u, cache.lookup i t = some u → cache'.lookup i t = some u :=
-iff.rfl
-
-lemma lt_iff_le_and_exists : cache < cache' ↔ cache ≤ cache' ∧
-  ∃ i t, cache.is_fresh i t ∧ cache'.is_cached i t :=
-begin
-  rw [lt_iff_le_and_ne],
-  simp only [ne.def, and.congr_right_iff],
-  intro h1,
-  refine ⟨λ h, by_contra (λ h', h (query_cache.ext (λ i t, _))), λ h h', _⟩,
-  { simp [is_cached_iff_not_is_fresh] at h',
-    by_cases ht : cache.is_fresh i t,
-    { calc cache.lookup i t = none : by simpa ... = cache'.lookup i t : by simpa using h' i t ht },
-    { rw [← is_cached_iff_not_is_fresh, is_cached_iff_exists_lookup_eq_some] at ht,
-      exact let ⟨u, hu⟩ := ht in hu.trans (h1 i t u hu).symm } },
-  { obtain ⟨i, t, hi⟩ := h,
-    rw [is_cached_iff_not_is_fresh, h'] at hi,
-    exact hi.2 hi.1 }
-end
-
-/-- The "smallest" element in the `query_cache` ordering is the empty cache. -/
-instance : order_bot (query_cache spec) :=
-{ bot := ∅,
-  bot_le := λ cache i t u h, (lookup_init_ne_some i t u h).elim }
-
-lemma bot_eq_init (spec : oracle_spec) : (⊥ : query_cache spec) = ∅ := rfl
-
-@[simp] lemma init_le : ∅ ≤ cache := bot_le
-
-lemma init_le' {cache : query_cache spec} : ∅ ≤ cache := bot_le
-
-@[simp] lemma init_lt_iff : ∅ < cache ↔ cache ≠ ∅ := bot_lt_iff_ne_bot
-
-@[simp] lemma le_init_iff : cache ≤ ∅ ↔ cache = ∅ := le_bot_iff
-
-@[simp] lemma not_lt_init : ¬ cache < ∅ := not_lt_bot
-
-@[simp] lemma inf_init : cache ⊓ ∅ = ∅ := inf_bot_eq
-
-@[simp] lemma init_inf : ∅ ⊓ cache = ∅ := bot_inf_eq
-
-lemma lookup_eq_some_of_le (h : cache ≤ cache')
-  (h' : cache.lookup i t = some u) : cache'.lookup i t = some u :=
-h i t u h'
-
-lemma lookup_eq_none_of_le (h : cache ≤ cache')
-  (h' : cache'.lookup i t = none) : cache.lookup i t = none :=
-by_contra (λ hs, let ⟨u, hu⟩ := (lookup_ne_none_iff_exists_lookup_eq_some _ _ _).1 hs in
-  (option.some_ne_none u ((h i t u hu).symm.trans h')))
-
-end order
 
 section cache_query
 
@@ -246,24 +200,21 @@ variables (i : spec.ι) (t : spec.domain i) (u : spec.range i)
 
 notation `[` i `,` t `↦` u `;` cache `]` := cache_query i t u cache
 
-@[simp] lemma lookup_cache_query (i' : spec.ι) (t' : spec.domain i') :
+lemma lookup_cache_query (i' : spec.ι) (t' : spec.domain i') :
   [i, t ↦ u; cache].lookup i' t' = if h : i = i' then
     (if h.rec t = t' then some (h.rec u) else cache.lookup i' t') else cache.lookup i' t' := rfl
 
-lemma lookup_cache_query_same_index (t' : spec.domain i) :
-  [i, t ↦ u; cache].lookup i t' = if t = t' then some u else cache.lookup i t' := by simp
+@[simp] lemma lookup_cache_query_same_index (t' : spec.domain i) :
+  [i, t ↦ u; cache].lookup i t' = if t = t' then some u else cache.lookup i t' :=
+by simp [lookup_cache_query]
 
-lemma lookup_cache_query_diff_index (i' : spec.ι) (t' : spec.domain i') (hi : i ≠ i') :
-  [i, t ↦ u; cache].lookup i' t' = cache.lookup i' t' := by simp [hi]
+@[simp] lemma lookup_cache_query_diff_index (i' : spec.ι) (t' : spec.domain i') (hi : i ≠ i') :
+  [i, t ↦ u; cache].lookup i' t' = cache.lookup i' t' := by simp [lookup_cache_query, hi]
 
 lemma lookup_cache_query_same_input : [i, t ↦ u; cache].lookup i t = some u := by simp
 
-lemma lookup_cache_query_diff_input (t' : spec.domain i) (ht : t ≠ t') :
+@[simp] lemma lookup_cache_query_diff_input (t' : spec.domain i) (ht : t ≠ t') :
   [i, t ↦ u; cache].lookup i t' = cache.lookup i t' := by simp [ht]
-
-lemma cache_query_monotone : monotone (cache_query i t u) :=
-λ cache cache' h i' t' u', by {simp only [lookup_cache_query],
-  split_ifs, exact id, exact h i' t' u', exact h i' t' u'}
 
 @[simp] lemma cache_query_ne_init : [i, t ↦ u; cache] ≠ ∅ :=
 ne_of_lookup_ne _ _ i t (by simp)
@@ -279,88 +230,45 @@ begin
   { simp }
 end
 
+lemma is_fresh_cache_query_same_index_iff (t' : spec.domain i) :
+  [i, t ↦ u; cache].is_fresh i t' ↔ cache.is_fresh i t' ∧ t ≠ t' := by simp
+
+lemma not_is_fresh_cache_query_same_input : ¬ [i, t ↦ u; cache].is_fresh i t := by simp
+
 @[simp] lemma is_cached_cache_query_iff (i' : spec.ι) (t' : spec.domain i') :
   [i, t ↦ u; cache].is_cached i' t' ↔ cache.is_cached i' t' ∨
     (if h : i = i' then h.rec t = t' else false) :=
-by {rw [is_cached_iff_not_is_fresh, is_fresh_cache_query_iff, not_and_distrib,
-  ← is_cached_iff_not_is_fresh], split_ifs; simp only [not_not, not_true] }
+begin
+  rw [← not_is_fresh_iff_is_cached, is_fresh_cache_query_iff,
+    not_and_distrib, not_is_fresh_iff_is_cached],
+  split_ifs; simp
+end
+
+lemma is_cached_cache_query_same_index_iff (t' : spec.domain i) :
+  [i, t ↦ u; cache].is_cached i t' ↔ cache.is_cached i t' ∨ t = t' := by simp
+
+lemma is_cached_cache_query_same_input : [i, t ↦ u; cache].is_cached i t := by simp
+
+lemma cache_query_inj_of_is_fresh (h : cache.is_fresh i t) (h' : cache'.is_fresh i t) :
+  [i, t ↦ u; cache] = [i, t ↦ u; cache'] ↔ cache = cache' :=
+begin
+  simp only [query_cache.ext_iff],
+  refine ⟨λ hc i' t', _, λ hc i' t', _⟩,
+  { by_cases hi : i = i',
+    { induction hi,
+      by_cases ht : t = t',
+      { simp [← ht, h, h'] },
+      { simpa [ht] using hc i t' } },
+    { simpa [hi] using hc i' t' } },
+  { by_cases hi : i = i',
+    { induction hi,
+      by_cases ht : t = t',
+      { simp [ht] },
+      { simpa [ht] using hc i t' } },
+    { simpa [hi] using hc i' t' } }
+end
 
 end cache_query
-
-section singleton
-
--- Special notation for cache containing a single value.
-notation `[` i `,` t `↦` u `]` := cache_query i t u ∅
-
-variables (i : spec.ι) (t : spec.domain i) (u : spec.range i)
-
-lemma lookup_singleton (i' : spec.ι) (t' : spec.domain i') :
-  [i, t ↦ u].lookup i' t' = if h : i = i' then
-    (if h.rec t = t' then some (h.rec u) else none) else none := rfl
-
-lemma lookup_singleton_same_index (t' : spec.domain i) :
-  [i, t ↦ u].lookup i t' = if t = t' then some u else none := by simp
-
-lemma lookup_singleton_same_input : [i, t ↦ u].lookup i t = some u := by simp
-
-lemma lookup_singleton_eq_some_iff (i' : spec.ι) (t' : spec.domain i') (u' : spec.range i') :
-  [i, t ↦ u].lookup i' t' = some u' ↔ ∃ (h : i = i'), h.rec t = t' ∧ h.rec u = u' :=
-begin
-  rw [lookup_singleton],
-  by_cases hi : i = i',
-  { induction hi,
-    by_cases ht : t = t'; simp [ht] },
-  { simp [hi] }
-end
-
-@[simp] lemma lookup_singleton_eq_some_iff_of_same_index (t' : spec.domain i) (u' : spec.range i) :
-  [i, t ↦ u].lookup i t' = some u' ↔ t = t' ∧ u = u' :=
-by simp [lookup_singleton_eq_some_iff, ite_eq_iff]
-
-lemma eq_singleton_iff : cache = [i, t ↦ u] ↔ cache ≤ [i, t ↦ u] ∧ cache ≠ ∅ :=
-begin
-  refine ⟨λ h, h.symm ▸ by simp, λ h, le_antisymm h.1 (λ i' t' u' h', _)⟩,
-  obtain ⟨i'', t'', u'', h''⟩ := (ne_init_iff' _).1 h.2,
-  obtain ⟨hi, ht, hu⟩ := (lookup_singleton_eq_some_iff _ _ _ _ _ _).1 (h.1 i'' t'' u'' h''),
-  obtain ⟨hi', ht', hu'⟩ := (lookup_singleton_eq_some_iff _ _ _ _ _ _).1 h',
-  induction hi, induction hi',
-  rwa [← ht', ← hu', ht, hu],
-end
-
-lemma singleton_ne_init : [i, t ↦ u] ≠ ∅ := cache_query_ne_init ∅ i t u
-
-@[simp] lemma le_singleton_iff : cache ≤ [i, t ↦ u] ↔ cache = ∅ ∨ cache = [i, t ↦ u] :=
-begin
-  rw [eq_singleton_iff, and_comm],
-  refine ⟨λ h, _, λ h, h.rec_on (λ h', le_of_eq_of_le h' (init_le _)) (λ h, h.2)⟩,
-  by_cases h' : cache = ∅,
-  { exact or.inl h' },
-  { exact or.inr ⟨h', h⟩ }
-end
-
-lemma le_singleton_iff_forall : cache ≤ [i, t ↦ u] ↔ ∀ i' t', cache.is_cached i' t' →
-  ∃ (h : i = i'), h.rec t = t' ∧ cache.lookup i' t' = some (h.rec u)  :=
-⟨λ h i' t' ht', let ⟨u', hu'⟩ := (cache.is_cached_iff_exists_lookup_eq_some _ _).1 ht' in
-  let ⟨hi, ht, hu⟩ := (lookup_singleton_eq_some_iff _ _ _ _ _ _).1 (h i' t' u' hu') in
-    ⟨hi, ht, hu.symm ▸ hu'⟩, λ h i' t' u' hu', (lookup_singleton_eq_some_iff _ _ _ _ _ _).2
-      (let ⟨hi, ht, hu⟩ := h i' t' (is_cached_of_lookup_eq_some _ hu') in
-        ⟨hi, ht, option.some_inj.1 (hu.symm.trans hu')⟩)⟩
-
-@[simp] lemma lt_singleton_iff : cache < [i, t ↦ u] ↔ cache = ∅ :=
-begin
-  rw [lt_iff_le_and_ne, le_singleton_iff, or_and_distrib_right,
-    and_not_self, or_false, and_iff_left_iff_imp],
-  exact λ h, h.symm ▸ (ne.symm (singleton_ne_init i t u))
-end
-
-@[simp] lemma singleton_le_iff : [i, t ↦ u] ≤ cache ↔ cache.lookup i t = some u :=
-begin
-  refine ⟨λ h, h i t u (lookup_singleton_same_input i t u), λ h i' t' u' h', _⟩,
-  obtain ⟨rfl, rfl, rfl⟩ := (lookup_singleton_eq_some_iff _ _ _ _ _ _).1 h',
-  exact h,
-end
-
-end singleton
 
 section drop_query
 
@@ -371,27 +279,23 @@ def drop_query (i : spec.ι) (t : spec.domain i) (cache : query_cache spec) :
 
 variables (i : spec.ι) (t : spec.domain i) (u : spec.range i)
 
-@[simp] lemma lookup_drop_query (i' : spec.ι) (t' : spec.domain i') :
+lemma lookup_drop_query (i' : spec.ι) (t' : spec.domain i') :
   (cache.drop_query i t).lookup i' t' = if h : i = i' then
     (if h.rec t = t' then none else cache.lookup i' t') else cache.lookup i' t' := rfl
 
-lemma lookup_drop_query_same_index (t' : spec.domain i) : (cache.drop_query i t).lookup i t' =
-  if t = t' then none else cache.lookup i t' := by simp
+@[simp] lemma lookup_drop_query_same_index (t' : spec.domain i) :
+  (cache.drop_query i t).lookup i t' = if t = t' then none else cache.lookup i t' :=
+by simp [lookup_drop_query]
 
-lemma lookup_drop_query_diff_index (i' : spec.ι) (t' : spec.domain i') (hi : i ≠ i') :
-  (cache.drop_query i t).lookup i' t' = cache.lookup i' t' := by simp [hi]
+@[simp] lemma lookup_drop_query_diff_index (i' : spec.ι) (t' : spec.domain i') (hi : i ≠ i') :
+  (cache.drop_query i t).lookup i' t' = cache.lookup i' t' := by simp [lookup_drop_query, hi]
 
 lemma lookup_drop_query_same_input : (cache.drop_query i t).lookup i t = none := by simp
 
 lemma lookup_drop_query_diff_input (t' : spec.domain i) (ht : t ≠ t'):
   (cache.drop_query i t).lookup i t' = cache.lookup i t' := by simp [ht]
 
-lemma drop_query_monotone : monotone (drop_query i t) :=
-λ cache cache' h i' t' u', by {simp only [lookup_drop_query],
-  split_ifs, exact id, exact h i' t' u', exact h i' t' u'}
-
-lemma drop_query_of_is_fresh (h : cache.is_fresh i t) :
-  cache.drop_query i t = cache :=
+@[simp] lemma drop_query_of_is_fresh (h : cache.is_fresh i t) : cache.drop_query i t = cache :=
 begin
   refine query_cache.ext (λ i t, _),
   simp [lookup_drop_query],
@@ -422,62 +326,154 @@ begin
     simp }
 end
 
+lemma is_fresh_drop_query_iff_same_index (t' : spec.domain i) :
+  (cache.drop_query i t).is_fresh i t' ↔ cache.is_fresh i t' ∨ t = t' := by simp
+
+lemma is_fresh_drop_query_iff_diff_index (i' : spec.ι) (t' : spec.domain i') (h : i ≠ i') :
+  (cache.drop_query i t).is_fresh i' t' ↔ cache.is_fresh i' t' := by simp [h]
+
+lemma is_fresh_drop_query_same_input : (cache.drop_query i t).is_fresh i t := by simp
+
+lemma is_fresh_drop_query_iff_diff_input (t' : spec.domain i) (h : t ≠ t') :
+  (cache.drop_query i t).is_fresh i t' ↔ cache.is_fresh i t' := by simp [h]
+
 @[simp] lemma drop_query_init : drop_query i t ∅ = ∅ := by simp
 
-@[simp] lemma drop_query_eq_init_iff : drop_query i t cache = ∅ ↔
-  ∃ u, cache ≤ [i, t ↦ u] :=
+end drop_query
+
+section drop_query_cache_query
+
+variables (i : spec.ι) (t : spec.domain i) (u : spec.range i)
+
+@[simp] lemma drop_query_cache_query (i' : spec.ι) (t' : spec.domain i') :
+  [i, t ↦ u; cache].drop_query i' t' = if h : i = i' then (if h.rec t = t' then cache.drop_query i' t'
+    else [i, t ↦ u; cache.drop_query i' t']) else [i, t ↦ u; cache.drop_query i' t'] :=
 begin
-  refine ⟨λ h, _, λ h, _⟩,
-  { by_cases h' : cache.is_fresh i t,
-    { rw [drop_query_of_is_fresh _ _ _ h'] at h,
-      exact ⟨default, h.symm ▸ init_le'⟩ },
-    { rw [← is_cached_iff_not_is_fresh, is_cached_iff_exists_lookup_eq_some] at h',
-      obtain ⟨u, hu⟩ := h',
-      refine ⟨u, λ i' t' u' hu', _⟩,
-      have := ((eq_init_iff _).1 h) i' t',
-      rw [is_fresh_drop_query_iff, ← lookup_eq_none_iff_is_fresh] at this,
-      refine this.rec_on (λ h', (option.some_ne_none u' (hu'.symm.trans h')).elim) _,
-      rintro ⟨rfl, rfl⟩,
-      exact (option.some_inj.1 (hu'.symm.trans hu)) ▸ (lookup_singleton_same_input _ _ _) } },
-  { obtain ⟨u, hu⟩ := h,
-    simp_rw [eq_init_iff, is_fresh_drop_query_iff, or_iff_not_imp_left,
-      ← is_cached_iff_not_is_fresh, is_cached_iff_exists_lookup_eq_some],
-    rintro i' t' ⟨u', hu'⟩,
-    obtain ⟨hi', ht', hu'⟩ := (lookup_singleton_eq_some_iff _ _ _ _ _ _).1 (hu i' t' u' hu'),
-    refine ⟨hi', ht'⟩ }
+  simp only [query_cache.ext_iff],
+  intros i'' t'',
+  by_cases hi : i = i',
+  { induction hi,
+    by_cases hi' : i = i'',
+    { induction hi',
+      by_cases ht : t = t',
+      { by_cases ht' : t' = t'',
+        { simp [ht, ht'] },
+        { simp [ht, ht'] } },
+      { by_cases ht' : t' = t'',
+        { simp [ht, ht', (ht' ▸ ht : t ≠ t'')] },
+        { simp [ht, ht'] } } },
+    { by_cases ht : t = t',
+      { simp [hi', ht] },
+      { simp [hi', ht] } } },
+  { by_cases hi' : i' = i'',
+    { induction hi',
+      simp [hi] },
+    { by_cases hi'' : i = i'',
+      { induction hi'',
+        simp [hi, hi'] },
+      { simp [hi, hi', hi''] } } }
 end
+
+lemma drop_query_cache_query_same_index (t' : spec.domain i) (u' : spec.domain i) :
+  [i, t ↦ u; cache].drop_query i t' =
+    if t = t' then cache.drop_query i t' else [i, t ↦ u; cache.drop_query i t'] := by simp
+
+lemma drop_query_cache_query_diff_index (i' : spec.ι) (t' : spec.domain i') (h : i ≠ i') :
+  [i, t ↦ u; cache].drop_query i' t' = [i, t ↦ u; cache.drop_query i' t'] := by simp [h]
 
 /-- Adding a value and then dropping it is the original cache if the added value was fresh,
 and otherwise is the result of dropping the same query from the original cache,
 since old cached values don't persist in the cache afterwords. -/
-@[simp] lemma drop_query_cache_query :
+@[simp] lemma drop_query_cache_query_same_input :
   [i, t ↦ u; cache].drop_query i t = if cache.is_fresh i t then cache else cache.drop_query i t :=
-sorry
+by by_cases h : cache.is_fresh i t; simp [h]
+
+lemma drop_query_cache_query_diff_input (t' : spec.domain i) (h : t ≠ t') :
+  [i, t ↦ u; cache].drop_query i t' = [i, t ↦ u; cache.drop_query i t'] := by simp [h]
+
+end drop_query_cache_query
+
+section cache_query_drop_query
 
 /-- Adding a value to a cache after removing a value for the same inputs is the same as just
 caching it into the original cache, since adding new values replaces old ones. -/
-@[simp] lemma cache_query_drop_query : [i, t ↦ u; cache.drop_query i t] = [i, t ↦ u; cache] :=
+@[simp] lemma cache_query_drop_query (i : spec.ι) (t : spec.domain i) (u : spec.range i) :
+  [i, t ↦ u; cache.drop_query i t] = [i, t ↦ u; cache] :=
 sorry
 
-end drop_query
+end cache_query_drop_query
 
-section order_cache_query_drop_query
+section singleton
+
+/-- Query cache with exactly one cached value given by the inputs -/
+def singleton (i : spec.ι) (t : spec.domain i) (u : spec.range i) := [i, t ↦ u; ∅]
+
+notation `[` i `,` t `↦` u `]` := singleton i t u
 
 variables (i : spec.ι) (t : spec.domain i) (u : spec.range i)
 
-@[simp] lemma le_cache_query_iff : cache ≤ [i, t ↦ u; cache'] ↔
-  (cache.is_fresh i t ∨ cache.lookup i t = some u) ∧
-    (cache.drop_query i t ≤ cache'.drop_query i t) :=
-begin
-  sorry,
-end
+lemma singleton.def : [i, t ↦ u] = [i, t ↦ u; ∅] := rfl
 
-@[simp] lemma cache_query_le_iff : [i, t ↦ u; cache] ≤ cache' ↔
-  cache'.lookup i t = some u ∧ cache.drop_query i t ≤ cache' :=
-begin
-  sorry
-end
+lemma lookup_singleton (i' : spec.ι) (t' : spec.domain i') :
+  [i, t ↦ u].lookup i' t' = if h : i = i' then
+    (if h.rec t = t' then some (h.rec u) else none) else none := rfl
 
-end order_cache_query_drop_query
+@[simp] lemma lookup_singleton_same_index (t' : spec.domain i) :
+  [i, t ↦ u].lookup i t' = if t = t' then some u else none := by simp [lookup_singleton]
+
+@[simp] lemma lookup_singleton_diff_index (i' : spec.ι) (t' : spec.domain i') (h : i ≠ i') :
+  [i, t ↦ u].lookup i' t' = none := by simp [lookup_singleton, h]
+
+lemma lookup_singleton_same_input :
+  [i, t ↦ u].lookup i t = some u := by simp
+
+@[simp] lemma lookup_singleton_diff_input (t' : spec.domain i) (h : t ≠ t') :
+  [i, t ↦ u].lookup i t' = none := by simp [h]
+
+lemma lookup_singleton_eq_some_iff (i' : spec.ι) (t' : spec.domain i')
+  (u' : spec.range i') : [i, t ↦ u].lookup i' t' = some u' ↔
+    ∃ (h : i = i'), h.rec t = t' ∧ h.rec u = u' :=
+by simp [lookup_singleton, dite_eq_iff, ite_eq_iff]
+
+lemma lookup_singleton_eq_some_iff_same_index (t' : spec.domain i) (u' : spec.range i) :
+  [i, t ↦ u].lookup i t' = some u' ↔ t = t' ∧ u = u' :=
+by simp [lookup_singleton_eq_some_iff, ite_eq_iff]
+
+lemma lookup_singleton_eq_some_iff_same_input (u' : spec.range i) :
+  [i, t ↦ u].lookup i t = some u' ↔ u = u' := by simp
+
+lemma singleton_ne_init : [i, t ↦ u] ≠ ∅ := cache_query_ne_init ∅ i t u
+
+@[simp] lemma is_fresh_singleton_iff (i' : spec.ι) (t' : spec.domain i') :
+  [i, t ↦ u].is_fresh i' t' ↔ if h : i = i' then h.rec t ≠ t' else true := by simp [singleton.def]
+
+lemma is_fresh_singleton_iff_same_index (t' : spec.domain i) :
+  [i, t ↦ u].is_fresh i t' ↔ t ≠ t' := by simp
+
+lemma is_fresh_singleton_diff_index (i' : spec.ι) (t' : spec.domain i') (h : i ≠ i') :
+  [i, t ↦ u].is_fresh i' t' := by simp [h]
+
+lemma not_is_fresh_singleton_same_input : ¬ [i, t ↦ u].is_fresh i t := by simp
+
+lemma is_fresh_singleton_diff_input (t' : spec.domain i) (h : t ≠ t') :
+  [i, t ↦ u].is_fresh i t' := by simp [h]
+
+@[simp] lemma drop_query_singleton (i' : spec.ι) (t' : spec.domain i') :
+  [i, t ↦ u].drop_query i' t' = if h : i = i' then (if h.rec t = t' then ∅
+    else [i, t ↦ u]) else [i, t ↦ u] :=
+by simp [singleton.def]
+
+lemma drop_query_singleton_same_index (t' : spec.domain i) :
+  [i, t ↦ u].drop_query i t' = if t = t' then ∅ else [i, t ↦ u] := by simp
+
+lemma drop_query_singleton_diff_index (i' : spec.ι) (t' : spec.domain i') (h : i ≠ i') :
+  [i, t ↦ u].drop_query i' t' = [i, t ↦ u] := by simp [h]
+
+lemma drop_query_singleton_same_input : [i, t ↦ u].drop_query i t = ∅ := by simp
+
+lemma drop_query_singleton_diff_input (t' : spec.domain i) (h : t ≠ t') :
+  [i, t ↦ u].drop_query i t' = [i, t ↦ u] := by simp [h]
+
+end singleton
 
 end query_cache
