src/computational_monads/simulation_semantics/constructions/logging/caching_oracle2.lean
@@ -1,0 +1,48 @@
+/-
+Copyright (c) 2022 Devon Tuma. All rights reserved.
+Released under Apache 2.0 license as described in the file LICENSE.
+Authors: Devon Tuma
+-/
+import computational_monads.simulation_semantics.constructions.logging.query_cache.get_or_else
+import computational_monads.simulation_semantics.simulate.monad
+
+/-!
+# Caching Simulation Oracle
+
+This file defines a `sim_oracle` that implements caching functionality.
+`cachingₛₒ` represents a simulator that caches fresh queries and returns the same value
+for any future queries, using a `query_cache` as an internal state for tracking this.
+
+This is used by being composed with other oracles, such as in `random_oracle`.
+-/
+
+open oracle_comp oracle_spec query_cache
+open prod (fst) (snd)
+
+variables {α β γ δ : Type} {spec spec' : oracle_spec}
+
+/-- Oracle for logging previous queries, and returning the same value for matching inputs.
+The `query_cache.get_or_else` function allows us to run a fallback for non-cached values. -/
+def cachingₛₒ {spec : oracle_spec} : sim_oracle spec spec (query_cache spec) :=
+{ default_state := ∅,
+  o := λ i ⟨t, cache⟩, cache.get_or_else i t (query i t) }
+
+namespace caching_oracle
+
+@[simp] lemma apply_eq (i : spec.ι) (x : spec.domain i × query_cache spec) :
+  cachingₛₒ i x = x.2.get_or_else i x.1 (query i x.1) := by cases x; refl
+
+@[simp_dist_equiv] lemma fst_map_apply_bind_apply_dist_equiv'
+  (i : spec.ι) (t : spec.domain i) (i' : spec.ι) (t' : spec.domain i') (cache : query_cache spec) :
+  do {x ← cachingₛₒ i' (t', cache), fst <$> cachingₛₒ i (t, x.2)} ≃ₚ
+    fst <$> cachingₛₒ i (t, cache) :=
+begin
+  refine trans (by apply fst_map_get_or_else_bind_get_or_else_dist_equiv) _,
+  split_ifs with hi ht,
+  induction hi,
+  simp [← ht],
+  pairwise_dist_equiv,
+  pairwise_dist_equiv,
+end
+
+end caching_oracle
