src/computational_monads/simulation_semantics/constructions/logging/query_cache/order.lean
@@ -1,0 +1,227 @@
+/-
+Copyright (c) 2023 Devon Tuma. All rights reserved.
+Released under Apache 2.0 license as described in the file LICENSE.
+Authors: Devon Tuma
+-/
+import computational_monads.simulation_semantics.constructions.logging.query_cache.basic
+import computational_monads.distribution_semantics.option
+
+/-!
+# Ordering on Query Caches
+
+This file defines a semilatice structure on `query_cache`, where `cache ≤ cache'` means
+that any cached value in `cache` has the same value in `cache'`,
+allowing any fresh value in `cache` to have any value (fresh or not) in `cache'`.
+
+We also define and `inf` operation and a `⊥` element (the empty cache).
+-/
+
+namespace query_cache
+
+open oracle_spec oracle_comp
+
+variables {α β γ : Type} {spec spec' : oracle_spec}
+
+
+/-- We say `cache ≤ cache'` for two query caches if every cached value in `cache` has the same
+value cached in `cache'`. For fresh values in `cache` the corresponding value can be anything.
+We also have an `inf` operation that only returns values cached in both original caches. -/
+instance : semilattice_inf (query_cache spec) :=
+{ le := λ cache cache', ∀ i t u, cache.lookup i t = some u → cache'.lookup i t = some u,
+  le_refl := λ cache i t u h, h,
+  le_trans := λ cache cache' cache'' h h' i t u h'', h' i t u (h i t u h''),
+  le_antisymm := λ cache cache' h' h, query_cache.ext (λ i t,
+    begin
+      by_cases hi : cache.lookup i t = none,
+      { by_cases hi' : cache'.lookup i t = none,
+        { rw [hi, hi'] },
+        { obtain ⟨u, hu⟩ := option.ne_none_iff_exists'.1 hi',
+          refine (option.some_ne_none u ((h i t u hu).symm.trans hi)).elim } },
+      { exact let ⟨u, hu⟩ := option.ne_none_iff_exists'.1 hi in (hu.trans (h' i t u hu).symm) }
+    end),
+  inf := λ cache cache' i t, if (cache.is_cached i t ∧ cache.lookup i t = cache'.lookup i t)
+    then cache.lookup i t else none,
+  inf_le_left := λ cache cache' i t u hu,
+    begin
+      by_cases h : cache.is_cached i t ∧ cache.lookup i t = cache'.lookup i t,
+      { exact (if_pos h).symm.trans hu },
+      { exact (option.some_ne_none u ((if_neg h).symm.trans hu).symm).elim }
+    end,
+  inf_le_right := λ cache cache' i t u hu,
+    begin
+      by_cases h : cache.is_cached i t ∧ cache.lookup i t = cache'.lookup i t,
+      { exact h.2 ▸ (if_pos h).symm.trans hu },
+      { exact (option.some_ne_none u ((if_neg h).symm.trans hu).symm).elim }
+    end,
+  le_inf := λ cache₁ cache₂ cache₃ h2 h3 i t u hu,
+    begin
+      by_cases h : cache₂.is_cached i t ∧ cache₂.lookup i t = cache₃.lookup i t,
+      { exact (if_pos h).trans (h2 i t u hu) },
+      { refine (not_and_distrib.1 h).rec (λ h, _) (λ h, _),
+        { exact (h (is_cached_of_lookup_eq_some _ (h2 i t u hu))).elim },
+        { exact (h ((h2 i t u hu).trans (h3 i t u hu).symm)).elim } }
+    end }
+
+variables (cache cache' : query_cache spec) (i : spec.ι) (t : spec.domain i) (u : spec.range i)
+
+lemma le.def : cache ≤ cache' ↔
+  ∀ i t u, cache.lookup i t = some u → cache'.lookup i t = some u := iff.rfl
+
+lemma inf.def : cache ⊓ cache' = λ i t,
+  if (cache.is_cached i t ∧ cache.lookup i t = cache'.lookup i t)
+    then cache.lookup i t else none := rfl
+
+lemma lookup_eq_some_of_le (h : cache ≤ cache')
+  (h' : cache.lookup i t = some u) : cache'.lookup i t = some u :=
+h i t u h'
+
+-- lemma lt_iff_le_and_exists : cache < cache' ↔ cache ≤ cache' ∧
+--   ∃ i t, cache.is_fresh i t ∧ cache'.is_cached i t :=
+-- begin
+--   rw [lt_iff_le_and_ne],
+--   simp only [ne.def, and.congr_right_iff],
+--   intro h1,
+--   refine ⟨λ h, by_contra (λ h', h (query_cache.ext (λ i t, _))), λ h h', _⟩,
+--   { simp [is_cached_iff_not_is_fresh] at h',
+--     by_cases ht : cache.is_fresh i t,
+--     { calc cache.lookup i t = none : by simpa ... = cache'.lookup i t : by simpa using h' i t ht },
+--     { rw [← is_cached_iff_not_is_fresh, is_cached_iff_exists_lookup_eq_some] at ht,
+--       exact let ⟨u, hu⟩ := ht in hu.trans (h1 i t u hu).symm } },
+--   { obtain ⟨i, t, hi⟩ := h,
+--     rw [is_cached_iff_not_is_fresh, h'] at hi,
+--     exact hi.2 hi.1 }
+-- end
+
+section bot
+
+/-- The "smallest" element in the `query_cache` ordering is the empty cache. -/
+instance : order_bot (query_cache spec) :=
+{ bot := ∅,
+  bot_le := λ cache i t u h, (lookup_init_ne_some i t u h).elim }
+
+lemma bot_eq_init (spec : oracle_spec) : (⊥ : query_cache spec) = ∅ := rfl
+
+@[simp] lemma init_le : ∅ ≤ cache := bot_le
+
+lemma init_le' {cache : query_cache spec} : ∅ ≤ cache := bot_le
+
+@[simp] lemma init_lt_iff : ∅ < cache ↔ cache ≠ ∅ := bot_lt_iff_ne_bot
+
+@[simp] lemma le_init_iff : cache ≤ ∅ ↔ cache = ∅ := le_bot_iff
+
+@[simp] lemma not_lt_init : ¬ cache < ∅ := not_lt_bot
+
+@[simp] lemma inf_init : cache ⊓ ∅ = ∅ := inf_bot_eq
+
+@[simp] lemma init_inf : ∅ ⊓ cache = ∅ := bot_inf_eq
+
+end bot
+
+section cache_query_drop_query
+
+lemma cache_query_monotone : monotone (cache_query i t u) :=
+λ cache cache' h i' t' u', by {simp only [lookup_cache_query],
+  split_ifs, exact id, exact h i' t' u', exact h i' t' u'}
+
+lemma drop_query_monotone : monotone (drop_query i t) :=
+λ cache cache' h i' t' u', by {simp only [lookup_drop_query],
+  split_ifs, exact id, exact h i' t' u', exact h i' t' u'}
+
+@[simp] lemma le_cache_query_self : cache ≤ [i, t ↦ u; cache] := sorry
+
+@[simp] lemma lt_cache_query_self_iff : cache < [i, t ↦ u; cache] ↔ cache.is_fresh i t := sorry
+
+@[simp] lemma drop_query_le_self : cache.drop_query i t ≤ cache := sorry
+
+@[simp] lemma drop_query_lt_self_iff : cache.drop_query i t < cache ↔ cache.is_cached i t := sorry
+
+@[simp] lemma drop_query_eq_init_iff_le_singleton : drop_query i t cache = ∅ ↔
+  ∃ u, cache ≤ [i, t ↦ u] :=
+sorry
+-- begin
+--   refine ⟨λ h, _, λ h, _⟩,
+--   { by_cases h' : cache.is_fresh i t,
+--     { rw [drop_query_of_is_fresh _ _ _ h'] at h,
+--       exact ⟨default, h.symm ▸ init_le'⟩ },
+--     { rw [← is_cached_iff_not_is_fresh, is_cached_iff_exists_lookup_eq_some] at h',
+--       obtain ⟨u, hu⟩ := h',
+--       refine ⟨u, λ i' t' u' hu', _⟩,
+--       have := ((eq_init_iff _).1 h) i' t',
+--       rw [is_fresh_drop_query_iff, ← lookup_eq_none_iff_is_fresh] at this,
+--       refine this.rec_on (λ h', (option.some_ne_none u' (hu'.symm.trans h')).elim) _,
+--       rintro ⟨rfl, rfl⟩,
+--       exact (option.some_inj.1 (hu'.symm.trans hu)) ▸ (lookup_singleton_same_input _ _ _) } },
+--   { obtain ⟨u, hu⟩ := h,
+--     simp_rw [eq_init_iff, is_fresh_drop_query_iff, or_iff_not_imp_left,
+--       ← is_cached_iff_not_is_fresh, is_cached_iff_exists_lookup_eq_some],
+--     rintro i' t' ⟨u', hu'⟩,
+--     obtain ⟨hi', ht', hu'⟩ := (lookup_singleton_eq_some_iff _ _ _ _ _ _).1 (hu i' t' u' hu'),
+--     refine ⟨hi', ht'⟩ }
+-- end
+
+@[simp] lemma le_cache_query_iff : cache ≤ [i, t ↦ u; cache'] ↔
+  (cache.is_fresh i t ∨ cache.lookup i t = some u) ∧
+    (cache.drop_query i t ≤ cache'.drop_query i t) :=
+begin
+  sorry,
+end
+
+@[simp] lemma cache_query_le_iff : [i, t ↦ u; cache] ≤ cache' ↔
+  cache'.lookup i t = some u ∧ cache.drop_query i t ≤ cache' :=
+begin
+  sorry
+end
+
+end cache_query_drop_query
+
+section singleton
+
+lemma eq_singleton_iff : cache = [i, t ↦ u] ↔ cache ≤ [i, t ↦ u] ∧ cache ≠ ∅ :=
+begin
+  sorry,
+  -- refine ⟨λ h, h.symm ▸ by simp, λ h, le_antisymm h.1 (λ i' t' u' h', _)⟩,
+  -- obtain ⟨i'', t'', u'', h''⟩ := (ne_init_iff_exists_eq_some _).1 h.2,
+  -- obtain ⟨hi, ht, hu⟩ := (lookup_singleton_eq_some_iff _ _ _ _ _ _).1 (h.1 i'' t'' u'' h''),
+  -- obtain ⟨hi', ht', hu'⟩ := (lookup_singleton_eq_some_iff _ _ _ _ _ _).1 h',
+  -- induction hi, induction hi',
+  -- rwa [← ht', ← hu', ht, hu],
+end
+
+
+@[simp] lemma le_singleton_iff : cache ≤ [i, t ↦ u] ↔ cache = ∅ ∨ cache = [i, t ↦ u] :=
+begin
+  rw [eq_singleton_iff, and_comm],
+  refine ⟨λ h, _, λ h, h.rec_on (λ h', le_of_eq_of_le h' (init_le _)) (λ h, h.2)⟩,
+  by_cases h' : cache = ∅,
+  { exact or.inl h' },
+  { exact or.inr ⟨h', h⟩ }
+end
+
+
+
+lemma le_singleton_iff_forall : cache ≤ [i, t ↦ u] ↔ ∀ i' t', cache.is_cached i' t' →
+  ∃ (h : i = i'), h.rec t = t' ∧ cache.lookup i' t' = some (h.rec u)  :=
+⟨λ h i' t' ht', let ⟨u', hu'⟩ := (cache.is_cached_iff_exists_lookup_eq_some _ _).1 ht' in
+  let ⟨hi, ht, hu⟩ := (lookup_singleton_eq_some_iff _ _ _ _ _ _).1 (h i' t' u' hu') in
+    ⟨hi, ht, hu.symm ▸ hu'⟩, λ h i' t' u' hu', (lookup_singleton_eq_some_iff _ _ _ _ _ _).2
+      (let ⟨hi, ht, hu⟩ := h i' t' (is_cached_of_lookup_eq_some _ hu') in
+        ⟨hi, ht, option.some_inj.1 (hu.symm.trans hu')⟩)⟩
+
+
+@[simp] lemma lt_singleton_iff : cache < [i, t ↦ u] ↔ cache = ∅ :=
+begin
+  rw [lt_iff_le_and_ne, le_singleton_iff, or_and_distrib_right,
+    and_not_self, or_false, and_iff_left_iff_imp],
+  exact λ h, h.symm ▸ (ne.symm (singleton_ne_init i t u))
+end
+
+@[simp] lemma singleton_le_iff : [i, t ↦ u] ≤ cache ↔ cache.lookup i t = some u :=
+begin
+  refine ⟨λ h, h i t u (lookup_singleton_same_input i t u), λ h i' t' u' h', _⟩,
+  obtain ⟨rfl, rfl, rfl⟩ := (lookup_singleton_eq_some_iff _ _ _ _ _ _).1 h',
+  exact h,
+end
+
+end singleton
+
+end query_cache
